Lustre/Parser/LustreParser.vy
@@ -24,7 +24,7 @@ Require Import List.
 Import ListNotations.
 %}
 
-%token<LustreAst.string * LustreAst.astloc> VAR_NAME
+%token<LustreAst.ident * LustreAst.astloc> VAR_NAME
 %token<LustreAst.constant * LustreAst.astloc> CONSTANT
 %token<LustreAst.astloc> TRUE FALSE
 %token<LustreAst.astloc> LEQ GEQ EQ NEQ LT GT PLUS MINUS STAR SLASH COLON COLONCOLON
@@ -53,14 +53,14 @@ Import ListNotations.
 %type<LustreAst.var_decls> var_decl
 %type<LustreAst.var_decls> var_decl_list
 %type<LustreAst.var_decls> local_var_decl
-%type<list LustreAst.string (* Reverse order *)> identifier_list
+%type<list LustreAst.ident (* Reverse order *)> identifier_list
 %type<LustreAst.type_name * LustreAst.astloc> type_name
 %type<LustreAst.preclock> declared_clock
 %type<LustreAst.clock> clock
 %type<LustreAst.var_decls> local_decl
 %type<LustreAst.var_decls> local_decl_list
 %type<LustreAst.var_decls (* Reverse order *)> parameter_list
-%type<list LustreAst.string> pattern
+%type<list LustreAst.ident> pattern
 %type<LustreAst.equation> equation
 %type<list LustreAst.equation> equations
 %type<unit> optsemicolon
@@ -281,7 +281,7 @@ expression:
 
 var_decl:
 | ids=identifier_list loc=COLON ty=type_name clk=declared_clock
-    { map (fun id=> (id, fst ty, clk, loc)) ids }
+    { map (fun id=> (id, (fst ty, clk, loc))) ids }
 
 var_decl_list:
 | vars=var_decl
@@ -327,11 +327,11 @@ declared_clock:
 | /* empty */
     { LustreAst.FULLCK LustreAst.BASE }
 | WHEN id=VAR_NAME
-    { LustreAst.WHENCK true (fst id) }
+    { LustreAst.WHENCK (fst id) true }
 | WHEN NOT id=VAR_NAME
-    { LustreAst.WHENCK false (fst id) }
+    { LustreAst.WHENCK (fst id) false }
 | WHENOT id=VAR_NAME
-    { LustreAst.WHENCK false (fst id) }
+    { LustreAst.WHENCK (fst id) false }
 | COLONCOLON clk=clock
     { LustreAst.FULLCK clk }
 
@@ -339,9 +339,9 @@ clock:
 | DOT
     { LustreAst.BASE }
 | clk=clock ON id=VAR_NAME
-    { LustreAst.ON clk true (fst id) }
+    { LustreAst.ON clk (fst id) true }
 | clk=clock ONOT id=VAR_NAME
-    { LustreAst.ON clk false (fst id) }
+    { LustreAst.ON clk (fst id) false }
 
 local_decl:
 | vd=local_var_decl
